pulse/examples/steel/NewCanon.fst
@@ -3,56 +3,56 @@ module NewCanon
 open FStar.Ghost
 open Steel.FractionalPermission
 open Steel.Memory
-open Steel.Effect.Atomic
-open Steel.Effect
+open Steel.SelEffect.Atomic
+open Steel.SelEffect
 
-assume val p (#n:int) (n2:int) : slprop
-assume val q (#n:int) (#n':int) (n2:int) : slprop
+assume val p (#n:int) (n2:int) : vprop
+assume val q (#n:int) (#n':int) (n2:int) : vprop
 
-assume val palloc (#n:int) (n2:int) : SteelT unit emp (fun _ -> p #n n2)
-assume val pwrite (#n:int) (#oldn:int) (newn:int) : SteelT unit (p #n oldn) (fun _ -> p #n newn)
+assume val palloc (#n:int) (n2:int) : SteelSelT unit emp (fun _ -> p #n n2)
+assume val pwrite (#n:int) (#oldn:int) (newn:int) : SteelSelT unit (p #n oldn) (fun _ -> p #n newn)
 
 assume val ref : Type0
-assume val ptr (_:ref) : slprop u#1
+assume val ptr (_:ref) : vprop
 
-assume val alloc (x:int)  : SteelT ref emp (fun y -> ptr y)
-assume val free (r:ref) : SteelT unit (ptr r) (fun _ -> emp)
-assume val read (r:ref) : SteelT int (ptr r) (fun _ -> ptr r)
+assume val alloc (x:int)  : SteelSelT ref emp (fun y -> ptr y)
+assume val free (r:ref) : SteelSelT unit (ptr r) (fun _ -> emp)
+assume val read (r:ref) : SteelSelT int (ptr r) (fun _ -> ptr r)
 
-let test_imp (x:int) : SteelT unit emp (fun _ -> p #1 1)  =
+let test_imp (x:int) : SteelSelT unit emp (fun _ -> p #1 1)  =
   let _ = palloc 0 in
   pwrite 1
 
-let test1 (x:int) : SteelT ref emp ptr =
+let test1 (x:int) : SteelSelT ref emp ptr =
   let y = alloc x in y
 
-let test2 (r:ref) : SteelT int (ptr r) (fun _ -> ptr r) =
+let test2 (r:ref) : SteelSelT int (ptr r) (fun _ -> ptr r) =
   let x = read r in
   x
 
-let test3 (r:ref) : SteelT int (ptr r) (fun _ -> ptr r)
+let test3 (r:ref) : SteelSelT int (ptr r) (fun _ -> ptr r)
   = let x = read r in
     let y = read r in
     x
 
-let test4 (r:ref) : SteelT ref (ptr r) (fun y -> ptr r `star` ptr y)
+let test4 (r:ref) : SteelSelT ref (ptr r) (fun y -> ptr r `star` ptr y)
   = let y = alloc 0 in
     y
 
-let test5 (r1 r2:ref) : SteelT ref (ptr r1 `star` ptr r2) (fun y -> ptr r1 `star` ptr r2 `star` ptr y)
+let test5 (r1 r2:ref) : SteelSelT ref (ptr r1 `star` ptr r2) (fun y -> ptr r1 `star` ptr r2 `star` ptr y)
   = let y = alloc 0 in
     y
 
-let test6 (r1 r2:ref) : SteelT unit (ptr r1 `star` ptr r2) (fun _ -> ptr r2 `star` ptr r1)
+let test6 (r1 r2:ref) : SteelSelT unit (ptr r1 `star` ptr r2) (fun _ -> ptr r2 `star` ptr r1)
   = let _ = read r1 in
     ()
 
-let test7 (a:unit) : SteelT ref emp (fun y -> ptr y) =
+let test7 (a:unit) : SteelSelT ref emp (fun y -> ptr y) =
   let x = alloc 0 in
   let v = read x in
   x
 
-let test8 (x:ref) : SteelT int (ptr x) (fun _ -> ptr x)
+let test8 (x:ref) : SteelSelT int (ptr x) (fun _ -> ptr x)
   = let v = read x in
     let y = alloc v in
     let v = read y in
@@ -61,30 +61,30 @@ let test8 (x:ref) : SteelT int (ptr x) (fun _ -> ptr x)
     assert (1 == 1);
     v
 
-let test_dep_frame () : SteelT ref emp (fun r -> ptr r)
+let test_dep_frame () : SteelSelT ref emp (fun r -> ptr r)
   = let r = alloc 0 in
     noop ();
     return r
 
 assume val reference (a:Type0) : Type0
-assume val pts_to (#a:Type0) (r:reference a) (p:perm) (v:erased a) : slprop u#1
-assume val rread (#a:Type) (#p:perm) (#v:erased a) (r:reference a) : SteelT (x:a{x == Ghost.reveal v}) (pts_to r p v) (fun _ -> pts_to r p v)
-assume val rwrite (#a:Type) (#v:erased a) (r:reference a) (v':a) : SteelT unit (pts_to r full_perm v) (fun _ -> pts_to r full_perm (Ghost.hide v'))
+assume val pts_to (#a:Type0) (r:reference a) (p:perm) (v:erased a) : vprop
+assume val rread (#a:Type) (#p:perm) (#v:erased a) (r:reference a) : SteelSelT (x:a{x == Ghost.reveal v}) (pts_to r p v) (fun _ -> pts_to r p v)
+assume val rwrite (#a:Type) (#v:erased a) (r:reference a) (v':a) : SteelSelT unit (pts_to r full_perm v) (fun _ -> pts_to r full_perm (Ghost.hide v'))
 
 assume val rwrite_alt (#a:Type) (#v:erased a) (r:reference a) (v'':erased a) (v':a{v'==Ghost.reveal v''})
-  : SteelT unit (pts_to r full_perm v) (fun _ -> pts_to r full_perm v'')
+  : SteelSelT unit (pts_to r full_perm v) (fun _ -> pts_to r full_perm v'')
 
-assume val r : slprop
+assume val r : vprop
 
 let read_write (#a:Type) (r0:reference a) (v0:erased a)
-  : SteelT unit (pts_to r0 full_perm v0 `star` r)
+  : SteelSelT unit (pts_to r0 full_perm v0 `star` r)
                 (fun _ -> r `star` pts_to r0 full_perm v0)
   = let u0 = rread r0 in
     rwrite_alt r0 v0 u0
 
 
 let swap (#a:Type) (r0 r1:reference a) (v0 v1:erased a)
-  : SteelT unit (pts_to r0 full_perm v0 `star` pts_to r1 full_perm v1)
+  : SteelSelT unit (pts_to r0 full_perm v0 `star` pts_to r1 full_perm v1)
                 (fun _ -> pts_to r0 full_perm v1 `star` pts_to r1 full_perm v0)
   = let u0 = rread r0 in
     let u1 = rread r1 in
@@ -92,11 +92,11 @@ let swap (#a:Type) (r0 r1:reference a) (v0 v1:erased a)
     rwrite_alt r1 v0 u0
 
 assume
-val rewrite_eq (#a:Type) (p:erased a -> slprop) (v0:erased a) (v1:erased a{v0 == v1})
-  : SteelT unit (p v0) (fun _ -> p v1)
+val rewrite_eq (#a:Type) (p:erased a -> vprop) (v0:erased a) (v1:erased a{v0 == v1})
+  : SteelSelT unit (p v0) (fun _ -> p v1)
 
 let swap2 (#a:Type) (r0 r1:reference a) (v0 v1:erased a)
-  : SteelT unit (pts_to r0 full_perm v0 `star` pts_to r1 full_perm v1)
+  : SteelSelT unit (pts_to r0 full_perm v0 `star` pts_to r1 full_perm v1)
                 (fun _ -> pts_to r0 full_perm v1 `star` pts_to r1 full_perm v0)
   = let u0 = rread r0 in
     let u1 = rread r1 in
@@ -105,39 +105,39 @@ let swap2 (#a:Type) (r0 r1:reference a) (v0 v1:erased a)
     rewrite_eq (pts_to r1 full_perm) (Ghost.hide u0) v0;
     rewrite_eq (pts_to r0 full_perm) (Ghost.hide u1) v1
 
-assume val alloc2 (x:int)  : SteelAtomicT ref Set.empty emp (fun y -> ptr y)
-assume val free2 (r:ref) : SteelAtomicT unit Set.empty (ptr r) (fun _ -> emp)
-assume val ghost_read (r:ref) : SteelGhostT (erased int) Set.empty (ptr r) (fun _ -> ptr r)
+assume val alloc2 (x:int)  : SteelSelAtomicT ref Set.empty emp (fun y -> ptr y)
+assume val free2 (r:ref) : SteelSelAtomicT unit Set.empty (ptr r) (fun _ -> emp)
+assume val ghost_read (r:ref) : SteelSelGhostT (erased int) Set.empty (ptr r) (fun _ -> ptr r)
 
-let test21 (x:int) : SteelAtomicT ref Set.empty emp ptr =
+let test21 (x:int) : SteelSelAtomicT ref Set.empty emp ptr =
   let y = alloc2 x in y
 
 [@expect_failure]
 // Cannot have two observable atomic computations
-let test22 (x:int) : SteelAtomicT unit Set.empty emp (fun _ -> emp) =
+let test22 (x:int) : SteelSelAtomicT unit Set.empty emp (fun _ -> emp) =
   let y = alloc2 x in
   free2 y
 
-let test23 (r:ref) : SteelGhostT (erased int) Set.empty (ptr r) (fun _ -> ptr r)
+let test23 (r:ref) : SteelSelGhostT (erased int) Set.empty (ptr r) (fun _ -> ptr r)
   = let x = ghost_read r in
     let y = ghost_read r in
     x
 
-let test24 (r:ref) : SteelAtomicT ref Set.empty (ptr r) (fun y -> ptr r `star` ptr y)
+let test24 (r:ref) : SteelSelAtomicT ref Set.empty (ptr r) (fun y -> ptr r `star` ptr y)
   = let y = alloc2 0 in
     y
 
-let test25 (r1 r2:ref) : SteelAtomicT ref Set.empty
+let test25 (r1 r2:ref) : SteelSelAtomicT ref Set.empty
     (ptr r1 `star` ptr r2) (fun y -> ptr r1 `star` ptr r2 `star` ptr y)
   = let y = alloc2 0 in
     y
 
 // Exercising subcomp on observability
-let test26 (r1 r2:ref) : SteelAtomicT unit Set.empty (ptr r1 `star` ptr r2) (fun _ -> ptr r2 `star` ptr r1)
+let test26 (r1 r2:ref) : SteelSelAtomicT unit Set.empty (ptr r1 `star` ptr r2) (fun _ -> ptr r2 `star` ptr r1)
   = let _ = ghost_read r1 in
     ()
 
-let test27 (a:unit) : SteelAtomicT ref Set.empty emp (fun y -> ptr y) =
+let test27 (a:unit) : SteelSelAtomicT ref Set.empty emp (fun y -> ptr y) =
   let x = alloc2 0 in
   let v = ghost_read x in
   return x
